HoneynetDefinitions.v
@@ -7,7 +7,7 @@ Require Import FileData.
 Require Import FileTypes.
 Require Import Tar.
 
-Variable gunzip: File->File.
+Variable gunzip: File->Disk->File.
 
 Local Open Scope bool.
 
@@ -16,7 +16,49 @@ Definition borland_rootkit (disk: Disk) :=
     isOnDisk file disk
     /\ isDeleted file
     /\ isGzip file disk
-    /\ Tar.looksLikeRootkit (gunzip file) disk.
+    /\ Tar.looksLikeRootkit (gunzip file disk) disk.
+
+Definition borland_rootkit_witness (disk: Disk) (file: File):=
+  isOnDisk file disk
+  /\ isDeleted file
+  /\ isGzip file disk
+  /\ Tar.looksLikeRootkit (gunzip file disk) disk.
+
+Definition borland_rootkit_witness_param (disk: Disk) (file gunzipped: File):=
+  isOnDisk file disk
+  /\ isDeleted file
+  /\ isGzip file disk
+  /\ Tar.looksLikeRootkit gunzipped disk.
+
+
+Lemma borland_rootkit_witness_impl :
+  forall (file: File) (disk: Disk),
+    borland_rootkit_witness disk file ->
+      borland_rootkit disk.
+Proof.
+  intros file disk H.
+  unfold borland_rootkit_witness in H.
+  unfold borland_rootkit.
+  exists file. assumption.
+Qed.
+
+Lemma borland_rootkit_fsubset :
+  forall (gzippedFile gunzipped: File) (disk:Disk),
+    gunzipped f⊆ (gunzip gzippedFile disk) ->
+      borland_rootkit_witness_param disk gzippedFile gunzipped ->
+        borland_rootkit_witness disk gzippedFile.
+Proof.
+  intros gzippedFile gunzipped disk subset H.
+  unfold borland_rootkit_witness_param in H.
+  unfold borland_rootkit_witness.
+  destruct H as [H0 H]. destruct H as [H1 H]. destruct H as [H2 H].
+  split. assumption.
+  split. assumption.
+  split. assumption.
+  apply looksLikeRootkit_fsubset with (1:=subset).
+  assumption.
+Qed.
+
 
 Definition borland_compute (disk: Disk) (file gunzipped: File)
   (filename1 filename2: string) :=
@@ -29,7 +71,7 @@ Definition borland_compute (disk: Disk) (file gunzipped: File)
 Lemma borland_reflection (disk: Disk) 
   (file gunzipped: File) (filename1 filename2: string) :
   borland_compute disk file gunzipped filename1 filename2 = true
-    -> (gunzip file) = gunzipped
+    -> (gunzip file disk) = gunzipped
       -> borland_rootkit disk.
 Proof.
   intros. unfold borland_compute in H.
@@ -44,19 +86,39 @@ Proof.
   rewrite H0. apply looksLikeRootkit_reflection in H1. auto.
 Qed.
 
-Lemma borland_rootkit_subset:
-  forall (sub super: Disk),
-    sub ⊆ super ->
-      borland_rootkit sub ->
-        borland_rootkit super.
+Lemma borland_witness_param_reflection:
+  forall (disk: Disk) (file gunzipped: File) (filename1 filename2: string),
+    borland_compute disk file gunzipped filename1 filename2 = true ->
+      borland_rootkit_witness_param disk file gunzipped.
 Proof.
-  intros sub super subset.
-  unfold borland_rootkit.
-  intros H.
-  destruct H as [file H]. exists file.
-  destruct H. destruct H0. destruct H1.
+  intros. unfold borland_compute in H.
+  apply Bool.andb_true_iff in H. destruct H.
+  apply Bool.andb_true_iff in H. destruct H.
+  apply Bool.andb_true_iff in H. destruct H.
+
+  unfold borland_rootkit_witness_param.
+  split. apply isOnDisk_reflection. auto.
+  split. unfold isDeleted. auto.
+  split. apply isGzip_reflection. auto.
+         apply looksLikeRootkit_reflection in H0. auto.
+Qed.
+
+Lemma borland_rootkit_witness_subset:
+  forall (sub super: Disk) (gzippedFile gunzipped: File),
+    borland_rootkit_witness_param sub gzippedFile gunzipped ->
+      sub ⊆ super ->
+        gunzipped f⊆ (gunzip gzippedFile super) ->
+            borland_rootkit super.
+Proof.
+  intros sub super gzippedFile gunzipped H subset fsubset.
+  unfold borland_rootkit_witness_param in H.
+  apply borland_rootkit_witness_impl with (file:=gzippedFile).
+  unfold borland_rootkit_witness.
+  destruct H as [HonDisk H]. destruct H as [Hdeleted H].
+  destruct H as [Hgzip Hlooks].
   split. apply isOnDisk_subset with (1:=subset). assumption.
   split. assumption.
   split. apply isGzip_subset with (1:=subset). assumption.
-         apply looksLikeRootkit_subset with (1:=subset). assumption.
+         apply looksLikeRootkit_subset with (1:=subset) in Hlooks.
+         apply looksLikeRootkit_fsubset with (1:=fsubset). assumption.
 Qed.
