FileIds.v
@@ -10,14 +10,12 @@ Local Open Scope N.
 
 Inductive FileId: Type :=
   | Ext2Id: N -> FileId
-  | TarId: FileId -> N -> FileId
   | MockId: list (N*Byte) -> FileId
 .
 
 Fixpoint eqb (lhs rhs: FileId) :=
   match (lhs, rhs) with
   | ((Ext2Id l), (Ext2Id r)) => N.eqb l r
-  | ((TarId lfs l), (TarId rfs r)) => (andb (eqb lfs rfs) (N.eqb l r))
   | ((MockId l), (MockId r)) => listN_Byte_eqb l r
   | _ => false
   end.
@@ -28,21 +26,11 @@ Proof.
   generalize rhs.
   induction lhs. 
     (* Ext2Id *)
-    destruct rhs0; 
-      [| simpl; intros; inversion H | simpl; intros; inversion H].
+    destruct rhs0; [| simpl; intros; inversion H].
     unfold eqb. intros. apply N.eqb_eq in H. rewrite H. reflexivity.
-    (* TarId *)
-    destruct rhs0; 
-      [simpl; intros; inversion H | | simpl; intros; inversion H].
-      intros. unfold eqb in H. 
-      apply Bool.andb_true_iff in H. destruct H.
-      apply N.eqb_eq in H0. rewrite H0.
-      apply IHlhs in H. rewrite H.
-      reflexivity.
     (* MockId *)
-    destruct rhs0; 
-      [simpl; intros; inversion H | simpl; intros; inversion H |].
-      intros. unfold eqb in H.
-      apply listN_Byte_eqb_reflection in H.
-      rewrite H. reflexivity.
+    destruct rhs0; [simpl; intros; inversion H | ].
+    intros. unfold eqb in H.
+    apply listN_Byte_eqb_reflection in H.
+    rewrite H. reflexivity.
 Qed.
